Vizing/new/Fan.lean
@@ -1,0 +1,164 @@
+import Vizing.new.EdgeColoring
+
+set_option linter.dupNamespace false
+set_option push_neg.use_distrib true
+
+namespace Fan
+open Graph
+open Nbhd
+open EdgeColoring
+
+/-
+
+A fan on (x, y) is a nonempty distinct list of vertices
+that are all adjacent to x such that
+the color of (x, F[i]) is free on F[i+1].
+
+Definition/axioms for a fan, and implementation of a function that creates
+a maximal fan from an edge (x, y).
+
+(Proof of maximality will happen once I define the notion of a subfan!)
+
+-/
+
+variable (n : Nat) (c : Nat) (G : Graph n) (C : EdgeColoring n c G)
+
+def colorAx (F : Array (Vertex n)) (x : Vertex n) :=
+  ∀ i, (h : i < (F.size - 1)) →
+  (color n c G C (x, F[i + 1]'(by exact Nat.add_lt_of_lt_sub h))) ∈
+  (freeColorsOn n c G C F[i])
+
+structure Fan (x y : Vertex n) where
+  val : Array (Vertex n)
+  nborsAx : val.toList ⊆ (nbhd n G x).val
+  nonemptyAx : val ≠ #[]
+  firstElemAx : val[0]'(by exact Array.size_pos_iff.mpr nonemptyAx) = y
+  colorAx : colorAx n c G C val x
+
+def default (x y : Vertex n) (h : present n G (x, y)) : Fan n c G C x y where
+  val := #[y]
+  nborsAx := by
+    simp
+    exact h.right
+  firstElemAx := by congr
+  nonemptyAx := by exact Array.ne_empty_of_size_eq_add_one rfl
+  colorAx := by simp [colorAx]
+
+def add (x y : Vertex n) (F : Array (Vertex n))
+  (nbors : List (Vertex n)) (h : F ≠ #[]) : Array (Vertex n) :=
+  match nbors with
+  | [] => F
+  | next :: rest =>
+    if color n c G C (x, next) ∈ freeColorsOn n c G C
+      (F.back (by exact Array.size_pos_iff.mpr h)) then
+    add x y (F.push next) rest (by exact Array.push_ne_empty) else
+    add x y F rest h
+
+theorem add_nborsAx (x y : Vertex n) (F : Array (Vertex n))
+  (nbors : List (Vertex n)) (hne : F ≠ #[]) (h : F.toList ⊆ nbhd n G x)
+  (hn : nbors ⊆ nbhd n G x) :
+  (add n c G C x y F nbors hne).toList ⊆ nbhd n G x := by
+  induction' nbors with z zs ih generalizing F
+  <;> simp [add]
+  · assumption
+  · split_ifs
+    all_goals apply List.cons_subset.mp at hn
+    · exact ih (F.push z) (by simp_all) (by simp_all) hn.right
+    · exact ih F hne h hn.right
+
+theorem add_nonemptyAx (x y : Vertex n) (F : Array (Vertex n))
+  (nbors : List (Vertex n)) (h : F ≠ #[]) :
+  (add n c G C x y F nbors h) ≠ #[] := by
+  induction' nbors with z zs ih generalizing F
+  <;> simp [add]
+  · assumption
+  · split_ifs
+    · exact ih (F.push z) (by exact Array.push_ne_empty)
+    · exact ih F h
+
+theorem add_firstElemAx (x y : Vertex n) (F : Array (Vertex n))
+  (nbors : List (Vertex n)) (hne : F ≠ #[])
+  (h : F[0]'(Array.size_pos_iff.mpr hne) = y) :
+  (add n c G C x y F nbors hne)[0]'(Array.size_pos_iff.mpr
+    (add_nonemptyAx n c G C x y F nbors hne)) = y := by
+  induction' nbors with z zs ih generalizing F
+  <;> simp [add]
+  · assumption
+  · split_ifs
+    all_goals apply ih
+    · rw [← h]
+      exact Array.getElem_push_lt (Array.size_pos_iff.mpr hne)
+    · assumption
+
+theorem add_colorAx (x y : Vertex n) (F : Array (Vertex n))
+  (nbors : List (Vertex n)) (hne : F ≠ #[]) (h : colorAx n c G C F x) :
+  colorAx n c G C (add n c G C x y F nbors hne) x := by
+  induction' nbors with z zs ih generalizing F
+  <;> simp [add]
+  exact h
+  split; all_goals rename_i h'
+  · apply ih (F.push z)
+    unfold colorAx at ⊢ h
+    simp only [Array.size_push, add_tsub_cancel_right]
+    intro i hi
+    by_cases hsize : i < F.size - 1
+    · have aux1 : (F.push z)[i]'(by simp [Array.size_push]; linarith) = F[i] := by
+        exact Array.getElem_push_lt hi
+      have aux2 : (F.push z)[i+1]'(by simp [Array.size_push]; linarith) = F[i+1] := by
+        apply Array.getElem_push_lt
+      simp_rw [aux1, aux2]
+      exact h i hsize
+    · have hi' : i = F.size - 1 := by
+        simp only [not_lt, tsub_le_iff_right] at hsize
+        apply Nat.lt_or_eq_of_le at hsize
+        rcases hsize with hsize | hsize
+        · linarith
+        · exact Nat.eq_sub_of_add_eq (Eq.symm hsize)
+      have aux1 : (F.push z)[i+1]'(by simp [Array.size_push]; linarith) = z := by
+        subst hi'
+        simp_rw [Nat.sub_add_cancel (Nat.one_le_of_lt hi)]
+        exact Array.getElem_push_eq
+      have aux2 : (F.push z)[i]'(by simp [Array.size_push]; linarith) = F.back := by
+        simp_rw [Array.getElem_push_lt (by exact hi), hi']
+        rfl
+      rw [aux1, aux2]
+      assumption
+  · exact ih F hne h
+
+def mkMaxFan (x y : Vertex n) (h : present n G (x, y)) : Array (Vertex n) :=
+  add n c G C x y (default n c G C x y h).val
+  ((nbhd n G x).val.erase y) (default n c G C x y h).nonemptyAx
+
+variable (x y : Vertex n)
+
+theorem mkMaxFan_nborsAx (hpres : present n G (x, y)) :
+  (mkMaxFan n c G C x y hpres).toList ⊆ (nbhd n G x).val := by
+  simp [mkMaxFan, default]
+  simp [present] at hpres
+  apply add_nborsAx
+  · simp
+    exact hpres.right
+  · exact List.erase_subset
+
+theorem mkMaxFan_nonemptyAx (x y : Vertex n) (hpres : present n G (x, y)) :
+  mkMaxFan n c G C x y hpres ≠ #[] := by
+  simp [mkMaxFan, default, add_nonemptyAx]
+
+theorem mkMaxFan_firstElemAx (x y : Vertex n) (hpres : present n G (x, y)) :
+  (mkMaxFan n c G C x y hpres)[0]'(by
+  exact Array.size_pos_iff.mpr (mkMaxFan_nonemptyAx n c G C x y hpres))
+  = y := by
+  simp [mkMaxFan, default, add_firstElemAx]
+
+theorem mkMaxFan_colorAx (x y : Vertex n) (hpres : present n G (x, y)) :
+  colorAx n c G C (mkMaxFan n c G C x y hpres) x := by
+  simp [mkMaxFan, (default n c G C x y hpres).colorAx, add_colorAx]
+
+def maximalFan (x y : Vertex n) (h : present n G (x, y)) : Fan n c G C x y where
+  val := mkMaxFan n c G C x y h
+  nborsAx := mkMaxFan_nborsAx n c G C x y h
+  firstElemAx := mkMaxFan_firstElemAx n c G C x y h
+  nonemptyAx := mkMaxFan_nonemptyAx n c G C x y h
+  colorAx := mkMaxFan_colorAx n c G C x y h
+
+end Fan
