Vizing/new/Subfan.lean
@@ -1,0 +1,24 @@
+import Vizing.new.Fan
+
+set_option linter.dupNamespace false
+set_option push_neg.use_distrib true
+-- set_option trace.profiler true
+
+namespace Subfan
+open Graph
+open Nbhd
+open EdgeColoring
+open Fan
+
+/-
+
+A fan on (x, y) is a nonempty distinct list of vertices
+that are all adjacent to x such that
+the color of (x, F[i]) is free on F[i+1].
+
+Definition/axioms for a fan, and implementation of a function that creates
+a maximal fan from an edge (x, y).
+
+-/
+
+end Subfan
